rename DijkstraMonad => DMonad

Dijkstra/DMonad.lean
@@ -3,15 +3,15 @@ import Dijkstra.OrderedMonad
 namespace Dijkstra
 
 /-! Dijkstra Monad -/
-class DijkstraMonad [Monad W] (D : ∀ (A : Type u), W A → Type v) where
+class DMonad [Monad W] (D : ∀ (A : Type u), W A → Type v) where
   ret : (a : A) → D A (pure a)
   bind : D A w₁ → ((x : A) → D B (w₂ x)) → D B (w₁ >>= w₂)
 
-open DijkstraMonad
+open DMonad
 
 variable {W} [OrderedMonad W] [LawfulMonad W]
 
-class LawfulDijkstraMonad (D : ∀ A, W A → Type) extends DijkstraMonad D where
+class LawfulDMonad (D : ∀ A, W A → Type) extends DMonad D where
   bind_ret {m : D A w} : bind m ret = cast (by simp) m
   bind_of_ret : bind (ret a) f = cast (by simp) (f a)
   bind_assoc : bind (bind m f) g = cast (by simp) (bind m (λx => bind (f x) g))
@@ -19,11 +19,11 @@ class LawfulDijkstraMonad (D : ∀ A, W A → Type) extends DijkstraMonad D wher
 class Weaken (D : ∀ A, W A → Type) where
   weaken (ma : D A w) (w' : W A) (h : w ≤ w') : D A w'
 
-class LawfulOrderedDijkstraMonad (D : ∀ A, W A → Type) extends LawfulDijkstraMonad D, Weaken D
+class LawfulOrderedDMonad (D : ∀ A, W A → Type) extends LawfulDMonad D, Weaken D
 
-namespace DijkstraMonad
+namespace DMonad
 
-@[simp, reducible] def verify {w : W A} [DijkstraMonad D] (ma : D A w) (w' : W A) := w ≤ w'
+@[simp, reducible] def verify {w : W A} [DMonad D] (ma : D A w) (w' : W A) := w ≤ w'
 
 @[simp, reducible] def ofEffObs [Monad M] (obs : ∀ {A}, M A → W A) := λ A w => { m : M A // obs m ≤ w }
 
@@ -32,7 +32,7 @@ instance instOfEffObs [Monad M] [LawfulMonad M] [LawfulOrderedMonad W]
     obs (return a) = return a)
   (obs_bind : ∀ {A B} {m : M A} {f : A → M B},
     obs (m >>= f) = (obs m) >>= (fun a => obs (f a)))
-  : LawfulOrderedDijkstraMonad (W := W) (ofEffObs obs) where
+  : LawfulOrderedDMonad (W := W) (ofEffObs obs) where
   ret a :=
     ⟨return a, by rw [obs_pure]; apply LawfulOrderedMonad.le_refl⟩
   bind
@@ -54,7 +54,7 @@ instance instOfEffObs [Monad M] [LawfulMonad M] [LawfulOrderedMonad W]
     | ⟨m,hm⟩ =>
       exact ⟨m, LawfulOrderedMonad.le_trans hm h⟩
 
-def toMonad (D : ∀ A, W A → Type) [DijkstraMonad D]
+def toMonad (D : ∀ A, W A → Type) [DMonad D]
   : Monad (fun A => Σ w, D A w) where
   pure a := ⟨return a, ret a⟩
   bind m f := ⟨m.1 >>= (fun a => (f a).1), bind m.2 (fun a => (f a).2)⟩
