Dijkstra/Pure.lean
@@ -1,0 +1,21 @@
+import Dijkstra.DMonad
+import Dijkstra.BaseSpecs.IDSpec
+
+namespace Dijkstra
+
+def DPure := DMonad.ofEffObs (M := Id) (W := IDSpec) (obs := pure)
+
+instance : LawfulOrderedDMonad (W := IDSpec) DPure :=
+  DMonad.instOfEffObs rfl rfl
+
+namespace Hidden
+
+def ret := @DMonad.ret _ _ (D := DPure)
+def bind := @DMonad.bind _ _ (D := DPure)
+
+def prog := bind (ret 5) (fun x => ret (x + 1))
+
+example : DMonad.verify prog (pure 6) := by
+  simp [DMonad.verify]
+  apply LawfulOrderedMonad.le_refl
+  
